LeanSubst/Ops.lean
@@ -72,6 +72,10 @@ theorem Action.hsmap_re [SubstMap S T] {σ : Subst T} {x : Nat} : (@re S x)[σ] 
 @[simp]
 theorem Action.hsmap_su [SubstMap S T] {σ : Subst T} {t : S} : (su t)[σ] = su t[σ] := by
   simp [SubstMap.smap]
+
+@[simp]
+theorem Subst.act_inner {f : Nat -> Action T} {x} : Subst.act { inner := f } x = f x := by
+  simp [act, SubstAction.act]
 ----------------------------------------------------------------------------------------------------
 ---- Identity
 ----------------------------------------------------------------------------------------------------
@@ -84,7 +88,7 @@ def Subst.id T : Subst T := ⟨λ x => re x⟩
 notation "+0" => Subst.id _
 
 @[simp]
-theorem Subst.id_action {x} : (id T).act x = re x := by simp [id, act]
+theorem Subst.id_action {x} : (id T).act x = re x := by simp [id, act, SubstAction.act]
 ----------------------------------------------------------------------------------------------------
 ---- Successor
 ----------------------------------------------------------------------------------------------------
@@ -97,7 +101,7 @@ def Subst.succ T : Subst T := ⟨λ x => re $ x + 1⟩
 notation "+1" => Subst.succ _
 
 @[simp]
-theorem Subst.succ_action {x} : (succ T).act x = re (x + 1) := by simp [succ, act]
+theorem Subst.succ_action {x} : (succ T).act x = re (x + 1) := by simp [succ, act, SubstAction.act]
 ----------------------------------------------------------------------------------------------------
 ---- Predecessor
 ----------------------------------------------------------------------------------------------------
@@ -110,7 +114,7 @@ def Subst.pred T : Subst T := ⟨λ x => re $ x - 1⟩
 notation "-1" => Subst.pred _
 
 @[simp]
-theorem Subst.pred_action {x} : (pred T).act x = re (x - 1) := by simp [pred, act]
+theorem Subst.pred_action {x} : (pred T).act x = re (x - 1) := by simp [pred, act, SubstAction.act]
 ----------------------------------------------------------------------------------------------------
 ---- Addition
 ----------------------------------------------------------------------------------------------------
@@ -128,7 +132,7 @@ theorem Ren.add_one : add T 1 = succ T := by simp [Ren.add, Ren.succ]
 def Subst.add T (k : Nat) : Subst T := ⟨λ x => re $ x + k⟩
 
 @[simp]
-theorem Subst.add_action {k x} : (add T k).act x = re (x + k) := by simp [add, act]
+theorem Subst.add_action {k x} : (add T k).act x = re (x + k) := by simp [add, act, SubstAction.act]
 
 @[simp]
 theorem Subst.add_zero : add T 0 = +0 := by simp [add, id]
@@ -152,7 +156,8 @@ theorem Ren.sub_one : sub T 1 = pred T := by simp [sub, pred]
 def Subst.sub T (k : Nat) : Subst T := ⟨λ x => re $ x - k⟩
 
 @[simp]
-theorem Subst.sub_action {k x} : (@sub T k).act x = re (x - k) := by simp [sub, act]
+theorem Subst.sub_action {k x} : (@sub T k).act x = re (x - k) := by
+  simp [sub, act, SubstAction.act]
 
 @[simp]
 theorem Subst.sub_zero : sub T 0 = +0 := by simp [sub, id]
@@ -182,10 +187,12 @@ def Subst.cons (a : Action T) (σ : Subst T) : Subst T := .mk λ n =>
 infixr:67 (name := Subst.cons_notation) " :: " => Subst.cons
 
 @[simp]
-theorem Subst.cons_action0 {a} {σ : Subst T} : (a::σ).act 0 = a := by simp [cons, act]
+theorem Subst.cons_action0 {a} {σ : Subst T} : (a::σ).act 0 = a := by
+  simp [cons, act, SubstAction.act]
 
 @[simp]
-theorem Subst.cons_action {a i} {σ : Subst T} : (a::σ).act (i + 1) = σ.act i := by simp [cons, act]
+theorem Subst.cons_action {a i} {σ : Subst T} : (a::σ).act (i + 1) = σ.act i := by
+  simp [cons, act, SubstAction.act]
 ----------------------------------------------------------------------------------------------------
 ---- Append
 ----------------------------------------------------------------------------------------------------
@@ -325,23 +332,23 @@ infixr:85 (name := Subst.compose_notation) " ∘ " => Subst.compose
 @[simp]
 theorem Subst.compose_action [SubstMap T T] {σ τ : Subst T} {x : Nat}
   : (σ ∘ τ).act x = (σ.act x)[τ]
-:= by simp [compose, act]
+:= by simp [compose, act, SubstAction.act]
 
 @[simp]
 theorem Subst.compose_pred_succ [SubstMap T T] : succ T ∘ pred T = id T := by
-  simp [succ, pred, id, compose, act]
+  simp [succ, pred, id, compose, act, SubstAction.act]
 
 @[simp]
 theorem Subst.compose_sub_add [SubstMap T T] {k} : add T k ∘ sub T k = id T := by
-  simp [sub, add, id, compose, act]
+  simp [sub, add, id, compose, act, SubstAction.act]
 
 @[grind =]
 theorem Subst.compose_add_succ_right [SubstMap T T] {k} : add T (k + 1) = add T k ∘ succ T := by
-  simp [add, succ, compose, act]; grind
+  simp [add, succ, compose, act, SubstAction.act]; grind
 
 @[grind =]
 theorem Subst.compose_add_succ_left [SubstMap T T] {k} : add T (k + 1) = succ T ∘ add T k := by
-  simp [add, succ, compose, act]; grind
+  simp [add, succ, compose, act, SubstAction.act]; grind
 
 def Subst.compose_ren_left : Ren T -> Subst T -> Subst T
 | r, τ => .mk λ n => τ.act (r.act n)
@@ -350,7 +357,7 @@ infixr:85 (name := Subst.compose_ren_left_notation) " ∘ " => Subst.compose_ren
 @[simp]
 theorem Subst.compose_ren_left_action {r : Ren T} {τ : Subst T} {x}
   : (r ∘ τ).act x = τ.act (r.act x)
-:= by simp [compose_ren_left, act]
+:= by simp [compose_ren_left, act, SubstAction.act]
 
 def Subst.compose_ren_right [RenMap T T] : Subst T -> Ren T -> Subst T
 | σ, r => .mk λ n => (σ.act n)⟨r⟩
@@ -359,7 +366,7 @@ infixr:85 (name := Subst.compose_ren_right_notation) " ∘ " => Subst.compose_re
 @[simp]
 theorem Subst.compose_ren_right_action [RenMap T T] {σ : Subst T} {r : Ren T} {x : Nat}
   : (σ ∘ r).act x = (σ.act x)⟨r⟩
-:= by simp [compose_ren_right, act]
+:= by simp [compose_ren_right, act, SubstAction.act]
 
 def Subst.hcompose [SubstMap S T] : Subst S -> Subst T -> Subst S
 | σ, τ => .mk λ n => (σ.act n)[τ]
@@ -368,7 +375,7 @@ infixr:85 " ◾ " => Subst.hcompose
 @[simp]
 theorem Subst.hcompose_action [SubstMap S T] {σ : Subst S} {τ : Subst T} {x : Nat}
   : (σ ◾ τ).act x = (σ.act x)[τ]
-:= by simp [hcompose, act]
+:= by simp [hcompose, act, SubstAction.act]
 
 def Subst.hcompose_ren [RenMap S T] : Subst S -> Ren T -> Subst S
 | σ, r => .mk λ n => (σ.act n)⟨r⟩
@@ -377,7 +384,7 @@ infixr:85 " ◾ " => Subst.hcompose_ren
 @[simp]
 theorem Subst.hcompose_ren_action [RenMap S T] {σ : Subst S} {r : Ren T} {x : Nat}
   : (σ ◾ r).act x = (σ.act x)⟨r⟩
-:= by simp [hcompose_ren, act]
+:= by simp [hcompose_ren, act, SubstAction.act]
 
 ----------------------------------------------------------------------------------------------------
 ---- Lift
@@ -430,12 +437,12 @@ def Subst.lift [RenMap T T] (σ : Subst T) (k : Nat := 1) : Subst T := .mk λ n 
 @[simp, grind <-]
 theorem Subst.lift_action_lt [RenMap T T] {σ : Subst T} {k i} (h : i < k)
   : (lift σ k).act i = re i
-:= by simp [lift, act]; grind
+:= by simp [lift, act, SubstAction.act]; grind
 
 @[simp, grind <-]
 theorem Subst.lift_action_ge [RenMap T T] {σ : Subst T} {k i} (h : i ≥ k)
   : (lift σ k).act i = (σ.act (i - k))⟨.add T k⟩
-:= by simp [lift, act]; grind
+:= by simp [lift, act, SubstAction.act]; grind
 ----------------------------------------------------------------------------------------------------
 ---- Action on variable list
 ----------------------------------------------------------------------------------------------------
@@ -447,11 +454,12 @@ instance : SubstAction T (List Nat) (List (Action T)) where
   act := Subst.act_list
 
 @[simp]
-theorem Subst.act_list_nil {σ : Subst T} : σ.act ([] : List Nat) = [] := by simp [act_list, act]
+theorem Subst.act_list_nil {σ : Subst T} : σ.act ([] : List Nat) = [] := by
+  simp [act_list, act, SubstAction.act]
 
 @[simp]
 theorem Subst.act_list_cons {σ : Subst T} {x} {ℓ : List Nat} : σ.act (x::ℓ) = σ.act x :: σ.act ℓ :=
-  by simp [act_list, act]
+  by simp [act_list, act, SubstAction.act]
 
 @[simp]
 theorem Subst.act_list_append {σ : Subst T} {x y : List Nat}
@@ -463,7 +471,7 @@ theorem Subst.act_list_append {σ : Subst T} {x y : List Nat}
 def Ren.to (r : Ren T) : Subst T := ⟨λ x => re (r.act x)⟩
 
 @[simp]
-theorem Ren.to_act {r : Ren T} {x} : (@to T r).act x = re (r.act x) := by simp [to, SubstAction.act]
+theorem Ren.to_act {r : Ren T} {x} : (@to T r).act x = re (r.act x) := by simp [to, Subst.act, SubstAction.act]
 
 @[simp]
 theorem Ren.to_id : (id T).to = .id T := by simp [to, id, Subst.id]
@@ -482,7 +490,7 @@ theorem Ren.to_sub {k} : (sub T k).to = .sub T k := by simp [to, sub, Subst.sub]
 
 @[simp]
 theorem Ren.to_lift [RenMap T T] {r : Ren T} {k} : (r.lift k).to = (@to T r).lift k := by
-  cases r; simp [to, lift, Subst.lift, SubstAction.act]; case _ act =>
+  cases r; simp [to, lift, Subst.lift, Subst.act, SubstAction.act]; case _ act =>
   funext; case _ x =>
   cases x; grind
   case _ n => cases Nat.decLt (n + 1) k <;> simp [ite]
@@ -492,6 +500,36 @@ theorem Ren.to_compose [RenMap T T] [SubstMap T T] {r1 r2 : Ren T}
   : @to T (r1 ∘ r2) = r1.to ∘ r2.to
 := by
   funext; case _ x =>
-  cases x <;> simp [to, compose, Subst.compose, SubstAction.act]
+  cases x <;> simp [to, compose, Subst.compose, Subst.act, SubstAction.act]
+----------------------------------------------------------------------------------------------------
+---- Range
+----------------------------------------------------------------------------------------------------
+def Ren.range : Nat -> Nat -> List Nat
+| _, 0 => []
+| s, e + 1 => if s ≤ e then (range s e).concat e else []
+
+infix:90 ".." => Ren.range
+
+@[simp]
+theorem Ren.range_same {n} : n..n = [] := by cases n <;> simp [range]
+
+@[simp, grind =]
+theorem Ren.range_ge_nil {s e} {h : s ≥ e} : s..e = [] := by
+  cases e <;> simp [range]; omega
+
+@[simp, grind =]
+theorem Ren.range_lt_cons {s e} {h : s < e} : s..e = s::(s.succ..e) := by
+  induction e
+  case _ => cases h
+  case _ n ih =>
+    cases Nat.decLt s n
+    case _ h2 =>
+      cases Nat.decEq s n
+      case _ h3 => exfalso; grind
+      case _ h3 => subst h3; simp [range]
+    case _ h2 =>
+      simp [range]
+      rw [ite_cond_eq_true, ite_cond_eq_true, ih (h := h2)]
+      all_goals grind
 
 end LeanSubst
