Examples/LambdaCalc.lean
@@ -1,6 +1,7 @@
 import LeanSubst
+open LeanSubst
 
-namespace LeanSubst.Examples.LambdaCalc
+namespace Examples.LambdaCalc
 
   inductive Term where
   | var : Nat -> Term
@@ -17,11 +18,11 @@ namespace LeanSubst.Examples.LambdaCalc
 
   @[simp, grind =]
   theorem Term.from_action_id {n} : from_action (+0.act n) = var n := by
-    simp [from_action, Subst.id]
+    simp [from_action]
 
   @[simp, grind =]
   theorem Term.from_action_succ {n} : from_action (+1.act n) = var (n + 1) := by
-    simp [from_action, Subst.succ]
+    simp [from_action]
 
   @[simp, grind =]
   theorem Term.from_acton_re {n} : from_action (re n) = var n := by simp [from_action]
@@ -81,15 +82,15 @@ namespace LeanSubst.Examples.LambdaCalc
     simp [SubstMap.smap]
 
   @[simp]
-  theorem Term.from_action_compose {x} {σ τ : Subst Term}
-    : (from_action (σ.act x))[τ] = from_action ((σ ∘ τ).act x)
+  theorem Term.from_action_compose {x : Nat} {σ τ : Subst Term}
+    : (from_action (Subst.act σ x))[τ] = from_action ((σ ∘ τ).act x)
   := by
-    simp [Term.from_action, Subst.compose]
+    simp [from_action, Subst.compose]
     generalize zdef : σ.act x = z
-    cases z <;> simp [Term.from_action]
+    cases z <;> simp [from_action]
 
   @[simp]
-  theorem Term.from_action_compose_ren {x} {σ : Subst Term} {r : Ren Term}
+  theorem Term.from_action_compose_ren {x : Nat} {σ : Subst Term} {r : Ren Term}
     : (from_action (σ.act x))⟨r⟩ = from_action ((σ ∘ r).act x)
   := by
     simp [Term.from_action]
@@ -111,4 +112,4 @@ namespace LeanSubst.Examples.LambdaCalc
   instance : SubstMapCompose Term Term where
     apply_compose := by subst_solve_compose
 
-end LeanSubst.Examples.LambdaCalc
+end Examples.LambdaCalc
